making the witnessed predicate ref-independent

lib/FStar.Monotonic.RRef.fst
@@ -1,6 +1,6 @@
 (*--build-config
     options:--admit_fsi FStar.Set --admit_fsi FStar.Map --admit_fsi FStar.HyperHeap;
-    other-files:FStar.Set.fsi FStar.Heap.fst map.fsi FStar.List.Tot.fst hyperHeap.fsi stHyperHeap.fst
+    other-files:FStar.Set.fsi FStar.Heap.fst map.fsi FStar.List.Tot.fst FStar.HyperHeap.fsi stHyperHeap.fst
  --*)
 module FStar.Monotonic.RRef
 open FStar
@@ -12,10 +12,6 @@ kind Reln (a:Type) = a -> a -> Type
 type monotonic (a:Type) (b:Reln a) =
   (forall x. b x x)                           (* reflexive *)
   /\ (forall x y z. b x y /\ b y z ==> b x z)   (* transitive *)
-
-type stable : #a:Type -> (a -> Type) -> Reln a -> Type =
-  fun (a:Type) (p:(a -> Type)) (b:Reln a) ->
-    (forall x y. p x /\ b x y ==> p y)
 
 private type m_rref (r:rid) (a:Type) (b:Reln a) = rref r a
  
@@ -34,7 +30,6 @@ let sel #r (a:Type) (b:Reln a) h m = HyperHeap.sel h m
 val upd: #r:rid -> #a:Type -> #b:Reln a -> h:t -> m_rref r a b -> a -> GTot t
 let upd r 'a 'b h m v = HyperHeap.upd h m v
 
-private type witnessed (#r:rid) (#a:Type) (#b:Reln a) (m:m_rref r a b) (p:(a -> Type)) = True
 
 val ralloc: #a:Type
           -> #b:Reln a
@@ -64,22 +59,21 @@ val write:#r:rid
               (ensures (assign_post (as_rref x) v))
 let write #r 'a 'b x v = x := v
 
-val witness:#r:rid
+type stable_on_t (#r:rid) (#a:Type) (#b:Reln a) (r:m_rref r a b) (p:(t -> Type)) = 
+  forall h0 h1. p h0 /\ b (sel h0 r) (sel h1 r) ==> p h1
+private type witnessed (p:(t -> Type)) = True
+
+val witness: #r:rid
           -> #a:Type
           -> #b:Reln a
           -> m:m_rref r a b
-          -> p:(a -> Type)
+          -> p:(t -> Type)
           -> ST unit
-                (requires (fun h0 -> p (sel h0 m) /\ stable p b))
-                (ensures (fun h0 _ h1 -> h0=h1 /\ witnessed m p))
-let witness #r (a:Type) (b:Reln a) m (p: a -> Type) = ()
+                (requires (fun h0 -> p h0 /\ stable_on_t m p))
+                (ensures (fun h0 _ h1 -> h0=h1 /\ witnessed p))
+let witness #r (#a:Type) (#b:Reln a) (m:m_rref r a b) (p: (t -> Type)) = ()
 
-assume val recall: #r:rid
-		-> #a:Type
-                -> #b:Reln a
-                -> m:m_rref r a b
-                -> p:(a -> Type)
+assume val recall: p:(t -> Type)
                 -> ST unit
-                      (requires (fun _ ->  witnessed m p))
-                      (ensures (fun h0 _ h1 -> h0=h1 /\ p (sel h1 m)))
-
+                      (requires (fun _ ->  witnessed p))
+                      (ensures (fun h0 _ h1 -> p h1))
